lakefile.lean
@@ -10,7 +10,7 @@ require mathlib from git
   "https://github.com/leanprover-community/mathlib4.git" @ "v4.32.1"
 
 require elevm from git
-  "https://github.com/skbaek/elevm.git" @ "c2a4a20d630dd6d8aef2d14429f40541a8e84c8b"
+  "https://github.com/skbaek/elevm.git" @ "a40871bc69df5159f6edc7fc7c3e928675b9f54d"
 
 @[default_target]
 lean_lib «Blanc» where
